# Homework #3

정보컴퓨터 공학과 201624623 홍윤영

#### 13.08 . Given the full joint distribution shown in Figure 13.3, calculate the following:

![스크린샷 2020-04-26 오전 10.32.48](/Users/Yoon/Library/Application Support/typora-user-images/스크린샷 2020-04-26 오전 10.32.48.png)

a. $$P(toothache)$$ 

​	$$P(toothache) = 0.108 + 0.012 + 0.016 + 0.064 = 0.2$$  

b. $$P(Cavity)$$

$$ P(Cavity) = 0.108 + 0.012 + 0.072 + 0.008 = 0.2$$

c. $$ P(Toothache | cavity)$$

$$P(Toothache|cavity) = (0.108 + 0.012)/0.2 = 0.6$$

d. $$P(Cavity | toothache ∨ catch)$$

$$P(Cavity|toothache \or catch) = (0.108+0.012 + 0.072)/0.416 = 0.461$$

#### 13.15 After your yearly checkup, the doctor has bad news and good news. The bad news is that you tested positive for a serious disease and that the test is 99% accurate (i.e., the probability of testing positive when you do have the disease is 0.99, as is the probability of testing negative when you don’t have the disease). The good news is that this is a rare disease, striking only 1 in 10,000 people of your age. Why is it good news that the disease is rare? What are the chances that you actually have the disease?

$$P(test|disease) = 0.99$$

$$P(\lnot test | \lnot disease )$$ = 0.99

$$P(disease) = 0.0001$$

$$P(disease|test) = {{P(test|disease) P(disease)} \over {P(test|disease)P(disease) + P(\lnot test| \lnot disease)P(\lnot disease)}} = 0.009804$$



#### 13.16 It is quite often useful to consider the effect of some specific propositions in the context of some general background evidence that remains fixed, rather than in the complete absence of information. The following questions ask you to prove more general versions of the product rule and Bayes’ rule, with respect to some background evidence e: a. Prove the conditionalized version of the general product rule:

#### a. P(X, Y | e) = P(X | Y, e)P(Y | e) 

$$P(X,Y|e) = {P(X,Y,e) \over P(e)}$$

$$P(X|Y,e)P(Y|e) = {P(X,Y,e) \over P(Y,e)} {P(Y,e) \over P(e)} = {P(X,Y,e) \over P(e)}$$

$$ \therefore P(X,Y|e) = P(X|Y,e)P(Y|e)$$

#### b. Prove the conditionalized version of Bayes’ rule in Equation (13.13)

![스크린샷 2020-04-26 오후 1.41.59](/Users/Yoon/Library/Application Support/typora-user-images/스크린샷 2020-04-26 오후 1.41.59.png)

$$P(X,Y|e) = P(Y|X,e)P(X|E) \\ P(Y|X,e)P(X|e) = P(X|Y,e)P(Y|e) \\  P(Y|X,e) = {P(X|Y,e)P(Y|e) \over P(X|e)}$$

#### 13.17  Show that the statement of conditional independence $$P(X, Y | Z) = P(X | Z)P(Y | Z)$$ is equivalent to each of the statements $$P(X | Y,Z) = P(X |Z)$$ and $$P(Y | X, Z) = P(Y | Z) $$.

$$P(X,Y|Z) = P(X|Z)P(Y|Z)$$

조건부 확률을 이용해 아래와 같이 정의

$$P(X,Y|Z) = P(X,Y,Z) P(Z) \\P(Y|Z) = P(Y,Z) P(Z) \\ P(X|Z) = P(X,Z) P(Z)$$

위의 식을 조합하면 아래와 같이 나옴

$${P(X,Y,Z)\over P(Z)} = P(X|Z) {P(Y,Z) \over P(Z)}$$

P(Z)를 곱하면 아래와 같다.

$$P(X,Y,Z) = P(X|Y,Z) P(Y,Z)$$

또 위의 식을 대입하여 전개하면 아래와 같다.

$${P(X|Y,Z)P(Y,Z) \over P(Z)} = P(X|Z) {P(Y,Z) \over P(Z)}$$

P(Z)를 곱하면 아래와 같다.

$$P(X|Y,Z) = P(X|Z)$$

위와 마찬가지의 과정을 거치면 반대로 거칠 경우

P(Y|X,Z) = P(Y|Z)

식이 나와서 참임을 증명할 수 있다.



#### 13.19 In this exercise, you will complete the normalization calculation for the meningitis example. First, make up a suitable value for P(s | ¬m), and use it to calculate unnormalized values for P(m | s) and P(¬m | s) (i.e., ignoring the P(s) term in the Bayes’ rule expression, Equation (13.14)). Now normalize these values so that they add to 1.

![스크린샷 2020-04-26 오후 2.11.29](/Users/Yoon/Library/Application Support/typora-user-images/스크린샷 2020-04-26 오후 2.11.29.png)

​																						Figure 13.14

$$P(s|\lnot m) = {P(¬m|s)P(s) \over P(\lnot m)} = {(1 − P(m|s))P(s) \over {1- P( m)}} = {0.9986 \times 0.01 \over  0.99998} = 0.009986199723994$$

$$P(s|m)P(m) = 0.7/50,000 = 0.000014$$

$$P(s|¬m)P(¬m) = 0.009986 × 0.99998 = 0.009985$$



$$P(m|s) =  { 0.000014 \over {0.000014 + 0.009985}} = 0.0014 $$

$$P(\lnot m|s) = 0.9986$$